 Knowing how signs behave is very important as equations become more complicated. The grammar presented here will be useful even in Calculus where signs will have to be distributed at times through an equation.

Where we have a -X in the tables below it is helpful to think of this as

$$
(-1) * x
$$

Doing this makes multiplying both sides of an equation by -1 intuitive where the sign of the equation needs to be changed.

**Table 2.1.1: Subtraction and addition of positive and negative terms**

|First Term|Operator|Second Term|Equals|
|----|----|----|----|
|X|+|X|$X+X = 2X$|
|X|+|-X|$X-X = 0$|
|X|-| X|$X-X = 0$|
|X|-| -X|$X+X=2X$|
|-X| -|-X|$-X+X=0$|
|-X| -|X|$-X-X=-2X$|
|-X|+| X|$-X+X = 0$|
|-X|+| -X|$-X-X = -2X$|

**Table 1.2.2: Division and multiplication of positive and negative terms**

|First Term|Operator|Second Term|Equals|
|----|----|----|----|
|Y|•|X|$YX$|
|Y|•|-X|$-YX$|
|Y|÷|X|$\frac{Y}{X}$|
|Y|÷|-X|$-\frac{Y}{X}$|
|-Y|÷|-X|$\frac{Y}{X}$|
|-Y|÷|X|$-\frac{Y}{X}$|
|-Y|•|X|$-YX$|
|-Y|•|-X|$YX$|

In the first table the first term can be thought of as your starting point on a number line and the combination of the operator and the sign of the second term determine the direction you travel on the line. The second table is less intuitive. Here the operator tells you only the overall form of the result (quotient or product). It the combined signs of the first and second term that determine the result.

When doing arithmetic or algebraic operations with signs it is useful to imagine that the term carries an invisible plus or minus one. Then you can determine what happens when this plus or minus one meets another plus or minus one.

**Example 2.1.1:**
We will now look at a simple example to illustrate the point. Here, although the first term has a negative sign, this just tells us the starting point. The operator and the second term are positive, so starting at $-x$, we are moving up by two.

$-x+2x\ \implies (-1)x+2•x\ \implies  2x-x \implies -x+x+x =x$

In fact there will be many occasions where simplifying an equation becomes considerably easier when you can manipulate signs of the terms effectively.

**Example 2.1.2:**
For example if we want to simplify:

$2x - y^2 - (3y - 6)^2 = 0$

**Distribute terms inside the parenthesis**

$(a)\ 2x - (1)y^2 - 1(3y - 6)^2=0$

$(b)\ 2x - y^2 −1⋅(9y^2−36y+36)=0$

**Combine like terms, rearrange and simplify**

$(a)\ -y^2 +2x - 9y^2 + 36y - 36 = 0$

$(b)\ -y^2 - 9y^2 + 36y + 2x - 36 = 0$

$(c)\ -10y^2 + 36y + 2x - 36 = 0$

Which gives us a fairly standard looking polynomial.

